Lecture 2

teaching/eutypes2018/ex/SumST.fst
@@ -4,26 +4,21 @@ open FStar.Ref
 open FStar.Mul
 
 // BEGIN: sum_rec
-let rec sum_rec (n:nat) = 
-  if n > 0 then n + sum_rec (n - 1) else 0
-
-let sum_tot (n:nat) = ((n+1) * n) / 2
-
-let rec sum_rec_correct (n:nat) : Lemma (sum_rec n = sum_tot n) = 
-  if n > 0 then sum_rec_correct (n - 1)
+let sum_tot (n:nat) = ((n+1) * n) / 2  (* equal to sum_rec, see 1st lecture exercises *)
 // END: sum_rec
 
-(* Exercise: strengthen spec of sum_st' so that sum_st verifies without admit *)
+(* Exercise: strengthen spec of sum_st' below so that sum_st verifies without admit *)
+
 // BEGIN: sum_st
 let rec sum_st' (r:ref nat) (n:nat) 
   : ST unit (requires (fun _ -> True))
-            (ensures  (fun _ _ _ -> True)) =
-  if n > 0 then (r := !r + n; 
-                 sum_st' r (n - 1))
+            (ensures  (fun _ _ _ -> True)) 
+  = if n > 0 then (r := !r + n; 
+                   sum_st' r (n - 1))
 
 let rec sum_st (n:nat) 
   : ST nat (requires (fun _ -> True))
-           (ensures  (fun h0 x h1 -> x == sum_rec n /\ 
+           (ensures  (fun h0 x h1 -> x == sum_tot n /\ 
                                      modifies !{} h0 h1))                                    
   = let r = alloc 0 in 
     sum_st' r n; 
